sketch pred that relates hidden to plain keys; and its necessary properties

proof/ktcore_proof/ktcore.v
@@ -5,10 +5,10 @@ From New.proof.github_com.sanjit_bhat.pav Require Import
   cryptoffi cryptoutil hashchain merkle safemarshal.
 
 From New.proof.github_com.sanjit_bhat.pav.ktcore_proof Require Import
-  serde sigpred.
+  common serde sigpred.
 
 Module ktcore.
-Import serde.ktcore sigpred.ktcore.
+Import common.ktcore serde.ktcore sigpred.ktcore.
 
 Section proof.
 Context `{hG: heapGS Σ, !ffi_semantics _ _, !globalsGS Σ} {go_ctx : GoContext}.
@@ -170,21 +170,6 @@ Proof.
   - by iFrame.
 Qed.
 
-Definition is_MapLabel vrf_pk uid ver map_label : iProp Σ :=
-  let enc := MapLabel.pure_enc (MapLabel.mk' uid ver) in
-  cryptoffi.is_vrf_out vrf_pk enc map_label.
-
-Lemma is_MapLabel_det pk uid ver map_label0 map_label1 :
-  is_MapLabel pk uid ver map_label0 -∗
-  is_MapLabel pk uid ver map_label1 -∗
-  ⌜map_label0 = map_label1⌝.
-Proof.
-  rewrite /is_MapLabel.
-  iIntros "#H0 #H1".
-  iDestruct (cryptoffi.is_vrf_out_det with "H0 H1") as %->.
-  done.
-Qed.
-
 Definition is_MapLabelProof vrf_pk uid ver proof : iProp Σ :=
   let enc := MapLabel.pure_enc (MapLabel.mk' uid ver) in
   cryptoffi.is_vrf_proof vrf_pk enc proof.
@@ -290,22 +275,6 @@ Proof.
   case_match.
   - iFrame.
   - iNamed "Hgenie0". iFrame "#".
-Qed.
-
-(* externalize [rand] bc some clients want to determ
-derive [map_val] from [kt_pk]. *)
-Definition is_MapVal kt_pk rand map_val : iProp Σ :=
-  let enc := CommitOpen.pure_enc (CommitOpen.mk' kt_pk rand) in
-  cryptoffi.is_hash (Some enc) map_val.
-
-Lemma is_MapVal_det pk rand map_val0 map_val1 :
-  is_MapVal pk rand map_val0 -∗
-  is_MapVal pk rand map_val1 -∗
-  ⌜map_val0 = map_val1⌝.
-Proof.
-  iIntros "#H0 #H1".
-  iDestruct (cryptoffi.is_hash_det with "H0 H1") as %->.
-  done.
 Qed.
 
 Lemma wp_GetMapVal sl_pk pk sl_rand rand :
