proof/ktcore_proof/sigpred.v
@@ -1,26 +1,134 @@
 From New.proof Require Import proof_prelude.
 From New.proof.github_com.sanjit_bhat.pav Require Import prelude.
 From New.proof.github_com.sanjit_bhat.pav Require Import
-  hashchain merkle safemarshal.
+  cryptoffi hashchain merkle safemarshal.
 
 From New.proof.github_com.sanjit_bhat.pav.ktcore_proof Require Import
-  serde.
+  common serde.
 
 Module ktcore.
-Import serde.ktcore.
+Import common.ktcore serde.ktcore.
 
 Module sigpred_cfg.
 Record t :=
   mk {
-    vrf: gname;
-    start_ep: gname;
-    links: gname;
+    vrf : gname;
+    (* the epoch of the first hist idx.
+    the auditor has no way of knowing if the server's digs start from epoch 0. *)
+    start_ep : gname;
+    (* the len offset after which auditor started monitoring. *)
+    audit_offset : gname;
+    hist : gname;
   }.
 End sigpred_cfg.
+
+(* gmap from uid's to list of pks (indexed by version). *)
+Definition keys_ty := gmap w64 (list $ list w8).
+
+(* FIXME: needed for lia to unify [length digs] terms where one has keys_ty and
+the other has its unfolding *)
+#[global] Hint Unfold keys_ty : word.
+
+Definition keys_sub : relation keys_ty := map_included (λ _, prefix).
 
 Section proof.
 Context `{hG: heapGS Σ, !ffi_semantics _ _, !globalsGS Σ} {go_ctx : GoContext}.
 Context `{!pavG Σ}.
+
+Definition decode_map_label odata :=
+  rem0 ← odata;
+  guard (length rem0 ≥ 8);;
+  let uid := le_to_u64 (take 8 rem0) in
+  let rem1 := drop 8 rem0 in
+  guard (length rem1 ≥ 8);;
+  let ver := le_to_u64 (take 8 rem1) in
+  Some (uid, uint.nat ver).
+
+Definition decode_map_val odata :=
+  rem0 ← odata;
+  guard (length rem0 ≥ 8);;
+  let pk_len := sint.nat (le_to_u64 (take 8 rem0)) in
+  let rem1 := drop 8 rem0 in
+  guard (length rem1 ≥ pk_len);;
+  let pk := take pk_len rem1 in
+  (* drop the remaining rand. we don't need that. *)
+  Some (pk).
+
+Definition is_decode_map_label vrf_pk map_label obj : iProp Σ :=
+  ∃ odata,
+  "#His_vrf_out" ∷ cryptoffi.is_vrf_out vrf_pk odata map_label ∗
+  "%Hdec" ∷ ⌜obj = decode_map_label odata⌝.
+
+Definition is_decode_map_val map_val obj : iProp Σ :=
+  ∃ odata,
+  "#His_hash" ∷ cryptoffi.is_hash odata map_val ∗
+  "%Hdec" ∷ ⌜obj = decode_map_val odata⌝.
+
+(* maybe change. *)
+Definition is_flat_keys vrf_pk hidden flat : iProp Σ :=
+  ∃ decoded,
+  "#Hdec" ∷ ([∗ list] kv;d ∈ map_to_list hidden;decoded,
+    is_decode_map_label vrf_pk kv.1 d.1 ∗
+    is_decode_map_val kv.2 d.2) ∗
+  "%Hflat" ∷ ⌜flat = omap (λ '(olabel, oval),
+    '(uid, ver) ← olabel;
+    pk ← oval;
+    Some (uid, ver, pk)) decoded⌝.
+
+(*
+structuring the hidden -> plain computation:
+- merkle labels are structurally unique.
+combined with is_vrf_out_inj, have unique (uid, ver).
+merkle val gives pk.
+- assemble into gmap uid (gmap ver pk).
+- now deal with each uid. gmap ver pk.
+- want to compute longest contiguous prefix.
+can write fixpoint for that, but with what max ver?
+size (gmap ver pk) is an easy over-approx.
+*)
+
+Definition is_plain_keys (vrf_pk : list w8) (hidden : gmap (list w8) (list w8))
+    (plain : keys_ty) : iProp Σ.
+Admitted.
+
+(* used by clients who agree across the same digs. *)
+Lemma is_plain_keys_det vrf_pk hidden plain0 plain1 :
+  is_plain_keys vrf_pk hidden plain0 -∗
+  is_plain_keys vrf_pk hidden plain1 -∗
+  ⌜plain0 = plain1⌝.
+Proof. Admitted.
+
+(* used by auditor.
+to prove, is_plain_keys can't require bijection. *)
+Lemma is_plain_keys_invert vrf_pk hidden :
+  ⊢ ∃ plain, is_plain_keys vrf_pk hidden plain.
+Proof. Admitted.
+
+(* used by auditor.
+maybe could be generalized? *)
+Lemma is_plain_keys_over_sub vrf_pk hidden0 hidden1 plain0 plain1 :
+  hidden0 ⊆ hidden1 →
+  is_plain_keys vrf_pk hidden0 plain0 -∗
+  is_plain_keys vrf_pk hidden1 plain1 -∗
+  ⌜keys_sub plain0 plain1⌝.
+Proof. Admitted.
+
+(* hidden is fully made up of contiguous versions.
+i.e., hidden and the computed plain are bijective. *)
+Definition is_contig (vrf_pk : list w8) (hidden : gmap (list w8) (list w8)) : iProp Σ.
+Admitted.
+
+(* used in server update. *)
+Lemma is_plain_keys_add vrf_pk hidden plain uid kt_pk label val rand :
+  let pks := plain !!! uid in
+  is_plain_keys vrf_pk hidden plain -∗
+  is_contig vrf_pk hidden -∗
+  is_MapLabel vrf_pk uid (length pks) label -∗
+  is_MapVal kt_pk rand val -∗
+  let hidden' := <[label:=val]>hidden in
+  let plain' := <[uid:=pks ++ [kt_pk]]>plain in
+  is_plain_keys vrf_pk hidden' plain' ∗ is_contig vrf_pk hidden'.
+Proof. Admitted.
 
 Definition sigpred_vrf γ (vrfPk : list w8) : iProp Σ :=
   "#Hshot" ∷ ghost_var γ.(sigpred_cfg.vrf) (□) vrfPk.
